Work on UTerminator.FWfM and friends

FreydSSA/Terminator/Fun/Basic.lean
@@ -6,12 +6,31 @@ variable {φ ν κ α} [Φ : InstSet φ (Ty α)]
   [DecidableEq ν] [DecidableEq κ] [DecidableEq α]
 
 inductive UTerminator.FWf : FCtx ν (Ty α) → UTerminator φ ν κ → FLCtx κ ν (Ty α) → Type _
-  | br : FLCtx.Wk (FLCtx.singleton ℓ ⟨Γ, A⟩) L → e.FWf p Γ A → (br ℓ e).FWf Γ L
-  | ite : e.FWf p Γ Ty.bool → s.FWf Γ L → t.FWf Γ L → (ite e s t).FWf Γ L
+  | br : FLCtx.Wk (FLCtx.singleton ℓ ⟨Γ, A⟩) L → e.FWf 1 Γ A → (br ℓ e).FWf Γ L
+  | ite : e.FWf 1 Γ Ty.bool → s.FWf Γ L → t.FWf Γ L → (ite e s t).FWf Γ L
 
+theorem UTerminator.FWf.allEq {Γ : FCtx ν (Ty α)} {t : UTerminator φ ν κ} : (dt dt' : t.FWf Γ L) → dt = dt'
+  | br _ de, br _ de' => by cases de.tyEq de'; cases de.allEq de'; rfl
+  | ite de ds dt, ite de' ds' dt' => by cases de.allEq de'; cases dt.allEq dt'; cases ds.allEq ds'; rfl
+
+-- TODO: research automatic generalization of stuff like this...
 inductive UTerminator.FWfM : FCtx ν (Ty α) → UTerminator φ ν κ → FLCtx κ ν (Ty α) → Type _
-  | br ℓ : e.FWf p Γ A → (br ℓ e).FWfM Γ (FLCtx.singleton ℓ ⟨Γ, A⟩)
-  | ite : e.FWf p Γ Ty.bool → s.FWfM Γ L → t.FWfM Γ K → L.Cmp K → (ite e s t).FWfM Γ (L.lsup K)
+  | br ℓ : e.FWf 1 Γ A → L' = FLCtx.singleton ℓ ⟨Γ, A⟩ → (br ℓ e).FWfM Γ L'
+  | ite : e.FWf 1 Γ Ty.bool → s.FWfM Γ L → t.FWfM Γ K → L.Cmp K → S = L.lsup K → (ite e s t).FWfM Γ S
+
+theorem UTerminator.FWfM.trgEq {Γ : FCtx ν (Ty α)} {t : UTerminator φ ν κ} : t.FWfM Γ L → t.FWfM Γ L' → L = L'
+  | br ℓ de rfl, br _ de' rfl => by cases de.tyEq de'; rfl
+  | ite _ ds dt _ rfl, ite _ ds' dt' _ rfl => by cases ds.trgEq ds'; cases dt.trgEq dt'; rfl
+
+theorem UTerminator.FWfM.allEq {Γ : FCtx ν (Ty α)} {t : UTerminator φ ν κ} : (dt dt' : t.FWfM Γ L) → dt = dt'
+  | br _ de _, br _ de' _ => by cases de.tyEq de'; cases de.allEq de'; rfl
+  | ite de ds dt h p, ite de' ds' dt' h' p' => by
+    cases ds.trgEq ds'; cases dt.trgEq dt'; cases de.allEq de'; cases ds.allEq ds'; cases dt.allEq dt'; rfl
+
+structure UTerminator.FWf' (Γ : FCtx ν (Ty α)) (t : UTerminator φ ν κ) (L : FLCtx κ ν (Ty α)) where
+  base : FLCtx κ ν (Ty α)
+  FWfM : t.FWfM Γ base
+  wk : base.Wk L
 
 --TODO: FWf', factorization, etc...
 
